@prefix : <http://schema.org/> .
@prefix rdf: <http://www.w3.org/1999/02/22-rdf-syntax-ns#> .
@prefix rdfs: <http://www.w3.org/2000/01/rdf-schema#> .

#
# Enumeration of Price categories (https://github.com/schemaorg/schemaorg/issues/2712)
#

:priceCategory a rdf:Property ;
  rdfs:label "priceCategory" ;
  :category "issue-2712" ;
  :isPartOf <http://pending.schema.org> ;
  :domainIncludes :CompoundPriceSpecification,
  	 :UnitPriceSpecification;
  :rangeIncludes :PriceCategoryEnumeration ;
  :source <https://github.com/schemaorg/schemaorg/issues/2712> ;
  rdfs:comment "Defines the price category for one of the prices associated with an offered product. Often, an offered product has pricing for different pricing categories, for example list price, a (temporary) sale price, or a manufacturer suggested retail price. If multiple prices are specified the /priceCategory property can be used to identify the category of each such specified price. If only a single price is present then this property is optional and by default /ListPrice value is assumed" .

:PriceCategoryEnumeration a rdfs:Class ;
  rdfs:label "PriceCategoryEnumeration" ;
  rdfs:subClassOf :Enumeration ;
  :category "issue-2712" ;
  :isPartOf <http://pending.schema.org> ;
  :source <https://github.com/schemaorg/schemaorg/issues/2712> ;
  rdfs:comment "Enumerates different price categories for an offer, for example list price and sale price." .

:ListPrice a :PriceCategoryEnumeration;
  rdfs:label "ListPrice" ;
  :category "issue-2712" ;
  :isPartOf <http://pending.schema.org> ;
  :source <https://github.com/schemaorg/schemaorg/issues/2712> ;
  rdfs:comment "Represents the list price (the price the product is actually advertised for) for an offered product." .

:SalePrice a :PriceCategoryEnumeration;
  rdfs:label "SalePrice" ;
  :category "issue-2712" ;
  :isPartOf <http://pending.schema.org> ;
  :source <https://github.com/schemaorg/schemaorg/issues/2712> ;
  rdfs:comment "Represents the sale price (usually active for a limited period) for an offered product." .
  
:MSRP a :PriceCategoryEnumeration;
  rdfs:label "MSRP" ;
  :category "issue-2712" ;
  :isPartOf <http://pending.schema.org> ;
  :source <https://github.com/schemaorg/schemaorg/issues/2712> ;
  rdfs:comment """Represents the manufacturer suggested retail price ("MSRP") for an offered product.""" .

:InvoicePrice a :PriceCategoryEnumeration;
  rdfs:label "InvoicePrice" ;
  :category "issue-2712" ;
  :isPartOf <http://pending.schema.org> ;
  :source <https://github.com/schemaorg/schemaorg/issues/2712> ;
  rdfs:comment "Represents the invoice price for an offered product." .
  
:MinimumAdvertisedPrice :PriceCategoryEnumeration;
  rdfs:label "MinimumAdvertisedPrice" ;
  :category "issue-2712" ;
  :isPartOf <http://pending.schema.org> ;
  :source <https://github.com/schemaorg/schemaorg/issues/2712> ;
  rdfs:comment """Represents the minimum advertised price ("MAP") (as dictated by the manufacturer) for an offered product.""" .
    